Update

ovn/src/ovn.rs
@@ -1,7 +1,218 @@
+/**************************/
+/*** Random Oracle file ***/
+/**************************/
+
 use hacspec_lib::*;
 
-mod schnorr;
-use schnorr::*;
+// INIT , QUERY (RO (RandomOracle) OracleParams)
+// Definition RO : package RO_locs [interface] RO_exports :=
+//   [package
+//     #def #[ INIT ] (_ : 'unit) : 'unit
+//     {
+//       #put queries_loc := emptym ;;
+//       ret Datatypes.tt
+//     } ;
+//     #def #[ QUERY ] (q : 'query) : 'random
+//     {
+//       queries ← get queries_loc ;;
+//       match queries q with
+//       | Some r =>
+//         ret r
+//       | None =>
+//         r ← sample uniform i_random ;;
+//         #put queries_loc := setm queries q r ;;
+//         ret r
+//       end
+//     }
+//   ].
+
+pub fn random_oracle_init(_ : ()) -> () {
+    ()
+}
+
+// #[derive(PartialEq, Eq, Clone, Copy)]
+// pub struct G{
+//     pub v : u32
+// }
+public_nat_mod!( //Custom Macro - defining a newtype with some functions - well defined macro's have library functions built in
+    type_name: G,
+    type_of_canvas: GCanvas,
+    bit_size_of_field: 384, //381 with 3 extra bits
+    modulo_value: "1a0111ea397fe69a4b1ba7b6434bacd764774b84f38512bf6730d2a0f6b0f6241eabfffeb153ffffb9feffffffffaaab" //0x1a0111ea397fe69a4b1ba7b6434bacd764774b84f38512bf6730d2a0f6b0f6241eabfffeb153ffffb9feffffffffaaab
+);
+
+// #[derive(PartialEq, Eq, Clone, Copy, Hash)]
+// pub struct Q {
+//     pub v : u32
+// }
+// Order of G
+public_nat_mod!( //Custom Macro - defining a newtype with some functions - well defined macro's have library functions built in
+    type_name: Q,
+    type_of_canvas: QCanvas,
+    bit_size_of_field: 384, //381 with 3 extra bits
+    modulo_value: "2566" // TODO Order of group G!
+);
+
+pub type Witness = Q;
+pub type Statement = G;
+pub type Message = G;
+pub type Challenge = Q;
+pub type Response =  Q;
+
+pub type Random = Challenge; // (Statement, Message);
+pub type Query = Challenge;
+
+// pub fn sample_uniform () -> Random {
+//     uniform_sample
+//     // (G{v: 1}, G{v: 1})// (Statement::ONE(), Message::ONE())
+// }
+
+use std::collections::HashMap;
+
+use std::hash::*;
+// use std::hash::{Hash, Hasher};
+impl Hash for Query {
+    fn hash<H: Hasher> (&self, state: &mut H) {
+
+    }
+}
+
+
+pub type QueriesType = HashMap<Query, Random>;
+// static ref QUERIES : HashMap<Query, Random> = HashMap::new();
+// chQuery  := 'fin #|Query|
+// chRandom := 'fin #|Random|
+pub fn random_oracle_query(mut QUERIES : QueriesType, q : Query, uniform_sample : Random) -> (QueriesType, Random) {
+    match QUERIES.get(&q)
+                 {
+        Some (r) => (QUERIES.clone(), r.clone()),
+        None => {
+            let r = uniform_sample;
+            QUERIES.insert(q, r);
+            (QUERIES, r)
+        }
+    }
+}
+
+/********************/
+/*** Schnorr file ***/
+/********************/
+
+// use hacspec_lib::*;
+// use std::collections::HashMap;
+
+// pub mod random_oracle;
+// use random_oracle::*;
+// type Transcript = (Message, Challenge, Response);
+
+// Sigma1.Sigma.RUN and Sigma1.Sigma.VERIFY: (Schnorr, RO (RandomOracle) OracleParams)
+// Definition Fiat_Shamir :
+//   package Sigma_locs
+//     [interface
+//       #val #[ INIT ] : 'unit → 'unit ;
+//       #val #[ QUERY ] : 'query → 'random
+//     ]
+//     [interface
+//       #val #[ VERIFY ] : chTranscript → 'bool ;
+//       #val #[ RUN ] : chRelation → chTranscript
+//     ]
+//   :=
+//   [package
+//     #def #[ VERIFY ] (t : chTranscript) : 'bool
+//     {
+//       #import {sig #[ QUERY ] : 'query → 'random } as RO_query ;;
+//       let '(h,a,e,z) := t in
+//       e ← RO_query (prod_assoc (h, a)) ;;
+//       ret (otf (Verify h a e z))
+//     } ;
+//     #def #[ RUN ] (hw : chRelation) : chTranscript
+//     {
+//       #import {sig #[ INIT ] : 'unit → 'unit } as RO_init ;;
+//       #import {sig #[ QUERY ] : 'query → 'random } as RO_query ;;
+//       let '(h,w) := hw in
+//       #assert (R (otf h) (otf w)) ;;
+//       a ← Commit h w ;;
+//       RO_init Datatypes.tt ;;
+//       e ← RO_query (prod_assoc (h, a)) ;;
+//       z ← Response h w a e ;;
+//       @ret choiceTranscript (h,a,e,z)
+//     }
+//   ].
+
+pub type Transcript = (Statement , Message , Challenge , Response);
+
+fn prod_assoc (sm : (Statement, Message)) -> // random_oracle::
+Query {
+    let (statement, message) = sm;
+    // Proof.
+    //   cbn. intros [statement message].
+    //   rewrite !card_prod.
+    //   apply mxvec_index. all: assumption.
+    // Qed.
+    // random_oracle::
+    Q::ONE()// {v: 1}
+    // random_oracle::Query::ONE()
+}
+
+// Verify_schamir
+fn verify (h : Statement, a : Message, e : Challenge, z : Response) -> bool {
+    // fto (g ^+ (otf z) == (otf a) * (otf h) ^+ (otf e))
+    false
+}
+
+pub fn fiat_shamir_verify(t : Transcript, uniform_sample : Random) -> bool {
+    let QUERIES = HashMap::new();
+    let (h,a,e,z) = t;
+    let (QUERIES, eu) = // random_oracle::
+    random_oracle_query (QUERIES, prod_assoc ((h, a)), uniform_sample);
+    // e <- eu;
+    // otf (
+    verify (h, a, e, z)
+    // )
+}
+
+pub type Relation = (Statement, Witness);
+
+fn Commit (h : Statement, w : Witness, uniform_sample : Random) -> Message {
+    // r ← sample uniform i_witness ;;
+    let r = uniform_sample;
+    // #put commit_loc := r ;;
+    let mut commit = r;
+    // ret (fto (g ^+ (otf r)))
+    // G{v: 1}
+    G::ONE()
+    // Message::ONE()
+}
+
+
+fn Response (h : Statement, w : Witness, a : Message, e : Challenge) -> Response {
+    // r ← get commit_loc ;;
+    // ret (fto (otf r + otf e * otf w))
+    Q::ONE()// {v: 1}
+    // Response::ONE()
+}
+
+pub fn fiat_shamir_run(hw : Relation, uniform_sample_1 : Random, uniform_sample_2 : Random) -> Transcript {
+    let QUERIES = HashMap::new();
+    // #import {sig #[ INIT ] : 'unit → 'unit } as RO_init ;;
+    // #import {sig #[ QUERY ] : 'query → 'random } as RO_query ;;
+    let (h,w) = hw;
+    // #assert (R (otf h) (otf w)) ;;
+    let a = Commit(h, w, uniform_sample_1);
+    // random_oracle::
+    random_oracle_init(());
+    let (QUERIES, eu) = // random_oracle::
+    random_oracle_query(QUERIES, prod_assoc((h, a)), uniform_sample_2);
+    let e = Q::ONE()// {v: 1}
+    ; // Challenge::ONE(); // Should be e <- eu
+    let z = Response (h, w, a, e);
+    (h,a,e,z)
+}
+
+// use hacspec_lib::*;
+
+// mod schnorr;
+// use schnorr::*;
 
 // (Exec_i i j m) ∘ (par ((P_i i b) ∘ (Sigma1.Sigma.Fiat_Shamir ∘ RO1.RO)) (Sigma1.Sigma.Fiat_Shamir ∘ RO1.RO))
 
@@ -45,23 +256,31 @@ use schnorr::*;
 //         }
 //     ].
 
-type Secret = schnorr::random_oracle::Q; // Zp_finComRingType (Zp_trunc #[g]);
-pub fn sample_uniform () -> Secret {
-    schnorr::random_oracle::Q{v: 1} // Secret::ONE()
-}
+type Secret = // schnorr::random_oracle::
+Q; // Zp_finComRingType (Zp_trunc #[g]);
+// pub fn sample_uniform () -> Secret {
+//     schnorr::random_oracle::Q{v: 1} // Secret::ONE()
+// }
 
-type public = schnorr::random_oracle::G;
-type public_key = (public, schnorr::Transcript); // (public, (schnorr::random_oracle::Message , schnorr::random_oracle::Challenge , schnorr::random_oracle::Response))
-fn p_i_init(_: ()) -> public_key {
+type public = // schnorr::random_oracle::
+G;
+type public_key = (public, // schnorr::
+                   Transcript); // (public, (schnorr::random_oracle::Message , schnorr::random_oracle::Challenge , schnorr::random_oracle::Response))
+fn p_i_init(_: (), uniform_sample : Secret, uniform_sample_R1 : // schnorr::random_oracle::
+            Random, uniform_sample_R2 : // schnorr::random_oracle::
+            Random) -> public_key {
     // #import {sig #[ Sigma1.Sigma.RUN ] : chRelation1 → chTranscript1} as ZKP ;;
     // #import {sig #[ Sigma1.Sigma.VERIFY ] : chTranscript1 → 'bool} as VER ;;
     // x ← sample uniform i_secret ;;
-    let x = sample_uniform();
+    let x = uniform_sample; // sample_uniform();
     // #put (skey_loc i) := x ;;
     // let y := (fto (g ^+ (otf x))) : public in
-    let y = schnorr::random_oracle::G{v: 1}; // public::ONE();
+    let y = // schnorr::random_oracle::
+    G::ONE() // {v: 1}
+    ; // public::ONE();
     // zkp ← ZKP (y, x) ;;
-    let zkp = schnorr::fiat_shamir_run((y, x));
+    let zkp = // schnorr::
+    fiat_shamir_run((y, x), uniform_sample_R1, uniform_sample_R2);
     (y, zkp)
 }
 
@@ -80,9 +299,10 @@ public_nat_mod!( //Custom Macro - defining a newtype with some functions - well 
 );
 
 type pid = N;
-use std::collections::HashMap;
+// use std::collections::HashMap;
 
-type public_keys = HashMap<pid, (public, schnorr::Transcript)>; // TODO
+type public_keys = HashMap<pid, (public, // schnorr::
+                                 Transcript)>; // TODO
 fn p_i_construct(m: public_keys) -> () {
     // #import {sig #[ Sigma1.Sigma.VERIFY ] : chTranscript1 → 'bool} as VER ;;
     // #assert (size (domm m) == n) ;;
@@ -101,7 +321,9 @@ fn p_i_vote(v: bool) -> public {
     // else
     //     let vote := (otf ckey ^+ skey * g ^+ (negb v)) in
     //     @ret 'public (fto vote)
-    schnorr::random_oracle::G{v: 1} // public::ONE()
+    // schnorr::random_oracle::
+    G::ONE()// {v: 1}
+    // public::ONE()
 }
 
 // Exec_i
@@ -123,18 +345,23 @@ fn p_i_vote(v: bool) -> public {
 //         }
 //     ]
 
-fn exec(v : bool) -> public {
+fn exec(v : bool,uniform_sample : Secret, uniform_sample_R1 : // schnorr::random_oracle::
+        Random, uniform_sample_R2 : // schnorr::random_oracle::
+        Random) -> public {
     // #import {sig #[ INIT ] : 'unit → 'public_key} as Init ;;
     // #import {sig #[ CONSTRUCT ] : 'public_keys → 'unit} as Construct ;;
     // #import {sig #[ VOTE ] : 'bool → 'public} as Vote ;;
     // #import {sig #[ Sigma1.Sigma.RUN ] : chRelation1 → chTranscript1} as ZKP ;;
     // pk ← Init Datatypes.tt ;;
     // x ← sample uniform i_secret ;;
-    let x = sample_uniform();
+    let x = uniform_sample;
     // let y := (fto (g ^+ (otf x))) : public in
-    let y = schnorr::random_oracle::G{v: 1}; // public::ONE();
+    let y = // schnorr::random_oracle::
+    G::ONE()// {v: 1}
+    ; // public::ONE();
     //     zkp ← ZKP (y, x) ;;
-    let zkp = schnorr::fiat_shamir_run((y, x));
+    let zkp = // schnorr::
+    fiat_shamir_run((y, x),uniform_sample_R1,uniform_sample_R2);
     // let m' := setm (setm m j (y, zkp)) i pk in
     //     Construct m' ;;
     // vote ← Vote v ;;
